shift-reset/core/env.v
@@ -1,7 +1,7 @@
 From shift_reset.core Require Import syntax ident.
 
-Fixpoint env_lookup (x : ident) (e : env) : option val :=
+Fixpoint env_find (x : ident) (e : env) : option val :=
   match e with
   | ENil => None
-  | ECons x' v e' => if ident_eqb x x' then Some v else env_lookup x e'
+  | ECons x' v e' => if ident_eqb x x' then Some v else env_find x e'
   end.
