shift-reset/interpreter/iheap.v
@@ -4,16 +4,16 @@ From shift_reset.core Require Import syntax loc.
 Record iheap : Type := IHeap { iheap_car : LocMap.t val; iheap_next_loc : loc }.
 
 Definition iheap_empty : iheap :=
-  IHeap gmap.empty loc_init.
+  IHeap gmap.empty loc_one.
 
 Definition iheap_alloc (v : val) (h : iheap) : iheap :=
-  let (m, l) := h in IHeap (LocMap.insert l v m) (loc_succ l).
+  let (m, l) := h in IHeap (LocMap.add l v m) (loc_succ l).
 
 Definition iheap_read (l : loc) (h : iheap) : option val :=
-  LocMap.lookup l (iheap_car h).
+  LocMap.find l (iheap_car h).
 
 Definition iheap_write (l : loc) (v : val) (h : iheap) : option iheap :=
-  let (m, l') := h in if LocMap.member l m then Some (IHeap (LocMap.insert l v m) l') else None.
+  let (m, l') := h in if LocMap.member l m then Some (IHeap (LocMap.add l v m) l') else None.
 
 Definition iheap_dealloc (l : loc) (h : iheap) : option iheap :=
-  let (m, l') := h in if LocMap.member l m then Some (IHeap (LocMap.delete l m) l') else None.
+  let (m, l') := h in if LocMap.member l m then Some (IHeap (LocMap.remove l m) l') else None.
